Functionally instantiate copy macros

books/projects/atomic-stobjs/constructors/copy.lisp
@@ -30,230 +30,39 @@
 (in-package "ATOMIC-STOBJS")
 (set-verify-guards-eagerness 2)
 
-(include-book "std/osets/top" :dir :system)
+(include-book "std/portcullis" :dir :system)
 
 (include-book "../utilities/top")
 (include-book "congruent")
 
-(deftheory set::theorems
-  (append
-   #!acl2'((:definition fast-alphorder)
-           (:executable-counterpart fast-alphorder)
-           (:type-prescription fast-alphorder)
-           (:executable-counterpart fast-lexorder)
-           (:type-prescription fast-lexorder)
-           (:rewrite fast-lexorder-is-lexorder)
-           (:executable-counterpart fast-<<)
-           (:type-prescription fast-<<)
-           (:executable-counterpart <<)
-           (:type-prescription <<)
-           (:rewrite <<-irreflexive)
-           (:rewrite <<-transitive)
-           (:rewrite <<-asymmetric)
-           (:rewrite <<-trichotomy)
-           (:rewrite <<-implies-lexorder)
-           (:rewrite fast-<<-is-<<))
+
+;;; `COUPLEDP'
+(encapsulate ()
+  (local
+    (defthm guard-lemma
+      (implies (character-listp x)
+               (character-listp (remove-equal a x)))))
 
-   #!set'((:executable-counterpart setp)
-          (:type-prescription setp)
-          (:type-prescription setp-type)
-          (:executable-counterpart emptyp)
-          (:type-prescription emptyp)
-          (:type-prescription emptyp-type)
-          (:executable-counterpart sfix)
-          (:type-prescription sfix)
-          (:executable-counterpart head)
-          (:type-prescription head)
-          (:executable-counterpart tail)
-          (:type-prescription tail)
-          (:executable-counterpart insert)
-          (:type-prescription insert)
-          (:executable-counterpart in)
-          (:type-prescription in)
-          (:type-prescription in-type)
-          (:executable-counterpart fast-subset)
-          (:type-prescription fast-subset)
-          (:executable-counterpart subset)
-          (:type-prescription subset)
-          (:type-prescription subset-type)
-          (:executable-counterpart fast-measure)
-          (:type-prescription fast-measure)
-          (:definition fast-union)
-          (:executable-counterpart fast-union)
-          (:type-prescription fast-union)
-          (:induction fast-union)
-          (:definition fast-intersect)
-          (:executable-counterpart fast-intersect)
-          (:type-prescription fast-intersect)
-          (:induction fast-intersect)
-          (:definition fast-intersectp)
-          (:executable-counterpart fast-intersectp)
-          (:type-prescription fast-intersectp)
-          (:induction fast-intersectp)
-          (:definition fast-difference)
-          (:executable-counterpart fast-difference)
-          (:type-prescription fast-difference)
-          (:induction fast-difference)
-          (:executable-counterpart delete)
-          (:type-prescription delete)
-          (:executable-counterpart union)
-          (:type-prescription union)
-          (:executable-counterpart intersect)
-          (:type-prescription intersect)
-          (:definition intersectp)
-          (:executable-counterpart intersectp)
-          (:type-prescription intersectp)
-          (:executable-counterpart difference)
-          (:type-prescription difference)
-          (:executable-counterpart cardinality)
-          (:type-prescription cardinality)
-          (:executable-counterpart halve-list-aux)
-          (:type-prescription halve-list-aux)
-          (:executable-counterpart halve-list)
-          (:type-prescription halve-list)
-          (:definition mergesort-exec)
-          (:executable-counterpart mergesort-exec)
-          (:type-prescription mergesort-exec)
-          (:induction mergesort-exec)
-          (:executable-counterpart mergesort)
-          (:type-prescription mergesort)
-          (:definition all)
-          (:executable-counterpart all)
-          (:type-prescription all)
-          (:induction all)
-          (:executable-counterpart subset-trigger)
-          (:type-prescription subset-trigger)
-          (:rewrite pick-a-point-subset-constraint-helper)
-          (:compound-recognizer sets-are-true-lists-compound-recognizer)
-          (:rewrite sets-are-true-lists-cheap)
-          (:rewrite tail-count)
-          (:linear tail-count)
-          (:rewrite head-count)
-          (:linear head-count)
-          (:built-in-clause tail-count-built-in)
-          (:built-in-clause head-count-built-in)
-          (:rewrite insert-insert)
-          (:rewrite sfix-produces-set)
-          (:rewrite tail-produces-set)
-          (:rewrite insert-produces-set)
-          (:rewrite insert-never-empty)
-          (:rewrite nonempty-means-set)
-          (:rewrite sfix-set-identity)
-          (:rewrite emptyp-sfix-cancel)
-          (:rewrite head-sfix-cancel)
-          (:rewrite tail-sfix-cancel)
-          (:rewrite insert-head)
-          (:rewrite insert-head-tail)
-          (:rewrite repeated-insert)
-          (:rewrite insert-sfix-cancel)
-          (:rewrite head-when-emptyp)
-          (:rewrite tail-when-emptyp)
-          (:rewrite insert-when-emptyp)
-          (:rewrite head-of-insert-a-nil)
-          (:rewrite tail-of-insert-a-nil)
-          (:rewrite sfix-when-emptyp)
-          (:rewrite not-in-self)
-          (:rewrite in-sfix-cancel)
-          (:rewrite never-in-empty)
-          (:rewrite in-set)
-          (:rewrite in-tail)
-          (:rewrite in-tail-or-head)
-          (:rewrite in-head)
-          (:rewrite head-unique)
-          (:rewrite insert-identity)
-          (:rewrite in-insert)
-          (:rewrite subset-insert-x)
-          (:rewrite subset-sfix-cancel-x)
-          (:rewrite subset-sfix-cancel-y)
-          (:rewrite emptyp-subset)
-          (:rewrite emptyp-subset-2)
-          (:rewrite subset-reflexive)
-          (:rewrite subset-insert)
-          (:rewrite subset-tail)
-          (:forward-chaining subset-tail)
-          (:rewrite weak-insert-induction-helper-1)
-          (:rewrite weak-insert-induction-helper-2)
-          (:rewrite weak-insert-induction-helper-3)
-          (:definition weak-insert-induction)
-          (:executable-counterpart weak-insert-induction)
-          (:type-prescription weak-insert-induction)
-          (:induction weak-insert-induction)
-          (:induction use-weak-insert-induction)
-          (:rewrite delete-delete)
-          (:rewrite delete-set)
-          (:rewrite delete-preserves-emptyp)
-          (:rewrite delete-in)
-          (:rewrite delete-sfix-cancel)
-          (:rewrite delete-nonmember-cancel)
-          (:rewrite repeated-delete)
-          (:rewrite delete-insert-cancel)
-          (:rewrite insert-delete-cancel)
-          (:rewrite subset-delete)
-          (:rewrite union-insert-x)
-          (:rewrite union-insert-y)
-          (:rewrite union-set)
-          (:rewrite union-sfix-cancel-x)
-          (:rewrite union-sfix-cancel-y)
-          (:rewrite union-emptyp-x)
-          (:rewrite union-emptyp-y)
-          (:rewrite union-emptyp)
-          (:rewrite union-in)
-          (:rewrite union-subset-x)
-          (:rewrite union-subset-y)
-          (:rewrite union-self)
-          (:rewrite union-associative)
-          (:rewrite union-outer-cancel)
-          (:rewrite intersect-delete-x)
-          (:rewrite intersect-delete-y)
-          (:rewrite intersect-set)
-          (:rewrite intersect-sfix-cancel-x)
-          (:rewrite intersect-sfix-cancel-y)
-          (:rewrite intersect-emptyp-x)
-          (:rewrite intersect-emptyp-y)
-          (:rewrite intersect-in)
-          (:rewrite intersect-subset-x)
-          (:rewrite intersect-subset-y)
-          (:rewrite intersect-self)
-          (:rewrite intersect-associative)
-          (:rewrite intersect-outer-cancel)
-          (:rewrite difference-set)
-          (:rewrite difference-sfix-x)
-          (:rewrite difference-sfix-y)
-          (:rewrite difference-emptyp-x)
-          (:rewrite difference-emptyp-y)
-          (:rewrite difference-in)
-          (:rewrite difference-subset-x)
-          (:rewrite subset-difference)
-          (:rewrite difference-insert-y)
-          (:rewrite difference-delete-x)
-          (:rewrite difference-preserves-subset)
-          (:type-prescription cardinality-type)
-          (:rewrite cardinality-zero-emptyp)
-          (:rewrite cardinality-sfix-cancel)
-          (:rewrite subset-cardinality)
-          (:linear subset-cardinality)
-          (:rewrite proper-subset-cardinality)
-          (:linear proper-subset-cardinality)
-          (:rewrite intersect-cardinality-x)
-          (:linear intersect-cardinality-x)
-          (:rewrite intersect-cardinality-y)
-          (:linear intersect-cardinality-y)
-          (:rewrite expand-cardinality-of-union)
-          (:rewrite expand-cardinality-of-difference)
-          (:rewrite intersect-cardinality-non-subset)
-          (:linear intersect-cardinality-non-subset)
-          (:rewrite intersect-cardinality-subset-2)
-          (:rewrite intersect-cardinality-non-subset-2)
-          (:rewrite mergesort-set)
-          (:rewrite in-mergesort-under-iff)
-          (:rewrite mergesort-set-identity)
-          (:rewrite insert-under-set-equiv)
-          (:rewrite delete-under-set-equiv)
-          (:rewrite union-under-set-equiv)
-          (:rewrite intersect-under-set-equiv)
-          (:rewrite difference-under-set-equiv)
-          (:rewrite mergesort-under-set-equiv)
-          (:congruence set-equiv-implies-equal-mergesort-1))))
+  (defun coupledp-fn (names acc)
+    (declare (xargs :guard (and (symbol-listp names)
+                                (symbol-list-listp acc))))
+    (if (atom names)
+        (revappend acc ())
+        (coupledp-fn (cdr names)
+                     (cons (let ((name (car names)))
+                             (list (symbolicate name (coerce (remove #\% (coerce (symbol-name name)
+                                                                                 'list))
+                                                             'string)
+                                                "-COUPLED-P")
+                                   name))
+                           acc)))))
+
+(defmacro coupledp (&rest names)
+  (declare (xargs :guard (symbol-listp names)))
+  (let ((expressions (coupledp-fn names ())))
+    (list 'case-split (if (null (cdr expressions))
+                          (car expressions)
+                          (cons 'and expressions)))))
 
 
 ;;;; `MAKE-VECTOR-COPY-EVENTS'
@@ -356,7 +165,7 @@
     `(progn
        (deflabel ,coupledp-begin)
 
-       (encapsulate ()
+       (with-books (("../lemmas/vector$a"))
 
          (local
            (deflabel prologue-begin))
@@ -388,10 +197,9 @@
          (local
            (in-theory
              (union-theories
-              (union-theories
-               (theory 'acl2::ground-zero)
-               (union-theories (theory ',vector$a-theorems)
-                               (theory ',vector$a-aggressive)))
+              (union-theories (theory 'acl2::ground-zero)
+                              (union-theories (theory ',vector$a-theorems)
+                                              (theory ',vector$a-aggressive)))
               (set-difference-theories (current-theory 'prologue-end)
                                        (current-theory 'prologue-begin)))))
 
@@ -440,38 +248,82 @@
 
                   (defthm ,coupledp-when-not-recognizer$a
                     (implies (not (,recognizer$a ,vector))
-                             (,coupledp ,vector)))
+                             (,coupledp ,vector))
+                    :hints
+                    (("Goal"
+                      :by (:functional-instance
+                           ,(if resizable
+                                'lem-vector$a::coupledp/resizable-when-not-recognizer/resizable
+                                'lem-vector$a::coupledp/fixed-when-not-recognizer/fixed)
+                           ,@fi-bindings))))
 
                   (defthm ,coupledp-of-creator$a
-                    (,coupledp (,creator$a)))
+                    (,coupledp (,creator$a))
+                    :hints
+                    (("Goal"
+                      :by (:functional-instance
+                           ,(if resizable
+                                'lem-vector$a::coupledp/resizable-of-creator
+                                'lem-vector$a::coupledp/fixed-of-creator)
+                           ,@fi-bindings))))
 
                   (defthm ,coupledp-of-fixer$a
                     (equal (,coupledp (,fixer$a ,vector))
-                           (,coupledp ,vector)))
+                           (,coupledp ,vector))
+                    :hints
+                    (("Goal"
+                      :by (:functional-instance
+                           ,(if resizable
+                                'lem-vector$a::coupledp/resizable-of-fixer/resizable
+                                'lem-vector$a::coupledp/fixed-of-fixer/fixed)
+                           ,@fi-bindings))))
 
-                  (defthm ,coupledp-of-resizer$a
-                    (implies (,coupledp ,vector)
-                             (,coupledp (,resizer$a length ,vector))))
+                  ,@(and resizable
+                         `((defthm ,coupledp-of-resizer$a
+                             (implies (,coupledp ,vector)
+                                      (,coupledp (,resizer$a length ,vector)))
+                             :hints
+                             (("Goal"
+                               :by (:functional-instance
+                                    lem-vector$a::coupledp/resizable-of-resizer/resizable
+                                    ,@fi-bindings))))))
 
                   (defthm ,element-coupled-p-of-accessor$a
                     (implies (,coupledp ,vector)
-                             (,element-coupled-p (,accessor$a ,index ,vector))))
-
-                  (defthm ,coupledp-of-updater$a
-                    (implies (and (,coupledp ,vector)
-                                  (,element-coupled-p ,element))
-                             (,coupledp (,updater$a ,index ,element ,vector)))
+                             (,element-coupled-p (,accessor$a ,index ,vector)))
+                    :rule-classes
+                    ((:rewrite :corollary
+                               (implies (coupledp ,vector)
+                                        (,element-coupled-p (,accessor$a ,index ,vector)))))
                     :hints
                     (("Goal"
-                      :cases ((< (nfix (,coupledp-witness (,updater ,index ,element ,vector)))
-                                 (,length$a ,vector)))
-                      :in-theory (disable ,coupledp
-                                          nfix)
-                      :expand (,coupledp (,updater$a ,index ,element ,vector)))))
+                      :by (:functional-instance
+                           ,(if resizable
+                                'lem-vector$a::element-coupled-p-of-accessor/resizable
+                                'lem-vector$a::element-coupled-p-of-accessor/fixed)
+                           ,@fi-bindings))))
+
+                  (defthm ,coupledp-of-updater$a
+                    (implies (,coupledp ,vector)
+                             (equal (,coupledp (,updater$a ,index ,element ,vector))
+                                    (if (<= ,(if resizable
+                                                 `(,length$a ,vector)
+                                                 default-length-name)
+                                            (nfix index))
+                                        t
+                                        (element-coupled-p value))))
+                    :hints
+                    (("Goal"
+                      :by (:functional-instance
+                           ,(if resizable
+                                'lem-vector$a::coupledp/resizable-of-updater/resizable
+                                'lem-vector$a::coupledp/fixed-of-updater/fixed)
+                           ,@fi-bindings))))
 
                   (in-theory
                     (disable ,coupledp))))
 
+         ;; `COPY-REC'
          (defun ,copy-rec (,index ,%vector ,vector)
            (declare (xargs :stobjs (,%vector ,vector)
                            :guard (and (= (,length ,%vector) (,length ,vector))
@@ -483,13 +335,6 @@
                     `(let ((,index (1- ,index)))
                        (stobj-let ((,element (,accessor ,index ,vector) ,updater))
                                   (,%vector)
-;;; TODO: `CONCRETE-ACCESSOR' gives error:
-;;; ```
-;;; HARD ACL2 ERROR in ASSERT$:  Assertion failed:
-;;; (ASSERT$ ACCESSOR$C (CONCRETE-ACCESSOR ACCESSOR$C (CDR TUPLES-LST)))
-;;; '''
-;;; when ACCESSOR is used instead of %ACCESSOR here (respectively UPDATER vs %UPDATER).
-;;; Is this a bug?
                                   (stobj-let ((,%element (,%accessor ,index ,%vector) ,%updater))
                                              (,%element)
                                              (,element-copy ,%element ,element)
@@ -500,29 +345,7 @@
                             (,%vector (,updater ,index ,element ,%vector)))
                        (,copy-rec ,index ,%vector ,vector)))))
 
-         (local
-           (defthm ,recognizer$a-of-copy-rec
-             (,recognizer$a (,copy-rec ,index ,%vector ,vector))))
-
-         (local
-           (defthm ,length$a-of-copy-rec
-             (equal (,length$a (,copy-rec ,index ,%vector ,vector))
-                    (,length$a ,%vector))))
-
-         (local
-           (defthm ,accessor$a-of-copy-rec
-             (implies ,(if element-coupled-p
-                           `(and (,coupledp ,vector)
-                                 (< (nfix i) (,length$a ,%vector)))
-                           `(< (nfix ,%index) (,length$a ,%vector)))
-                      (equal (,accessor$a ,%index (,copy-rec ,index ,%vector ,vector))
-                             (if (< (nfix ,%index) (nfix ,index))
-                                 (,accessor$a ,%index ,vector)
-                                 (,accessor$a ,%index ,%vector))))))
-
-         (in-theory
-           (disable ,copy-rec))
-
+         ;; `COPY'
          (defun ,copy (,%vector ,vector)
            (declare (xargs :stobjs (,%vector ,vector)))
            (let* ((length (,length ,vector))
@@ -534,36 +357,65 @@
          (table copy ',vector ',copy)
 
          (defthm ,recognizer$a-of-copy
-           (,recognizer$a (,copy ,%vector ,vector)))
+           (,recognizer$a (,copy ,%vector ,vector))
+           :hints
+           (("Goal"
+             :by (:functional-instance
+                  ,(if resizable
+                       'lem-vector$a::recognizer/resizable-of-copy/resizable
+                       'lem-vector$a::recognizer/fixed-of-copy/fixed)
+                  ,@fi-bindings-with-copy))))
 
-         (defthm ,length$a-of-copy
-           (equal (,length$a (,copy ,%vector ,vector))
-                  (,length$a ,vector)))
+         (defthm ,copy-of-fixer$a-1
+           (equal (copy (fixer$a %vector) vector)
+                  (copy %vector vector))
+           :hints
+           (("Goal"
+             :by (:functional-instance
+                  ,(if resizable
+                       'lem-vector$a::copy/resizable-of-fixer/resizable-1
+                       'lem-vector$a::copy/fixed-of-fixer/fixed-1)
+                  ,@fi-bindings-with-copy))))
 
-         (local
-           (defthm ,accessor$a-of-copy
-             (implies ,(if element-coupled-p
-                           `(and (,coupledp ,vector)
-                                 (< (nfix ,index) (,length$a ,vector)))
-                           `(< (nfix ,index) (,length$a ,vector)))
-                      (equal (,accessor$a ,index (,copy ,%vector ,vector))
-                             (,accessor$a ,index ,vector)))))
+         (defthm copy-of-fixer$a-2
+           (equal (copy %vector (fixer$a vector))
+                  (copy %vector vector))
+           :hints
+           (("Goal"
+             :by (:functional-instance
+                  ,(if resizable
+                       'lem-vector$a::copy/resizable-of-fixer/resizable-2
+                       'lem-vector$a::copy/fixed-of-fixer/fixed-2)
+                  ,@fi-bindings-with-copy))))
+
+         ,@(and resizable
+                `((defthm ,length$a-of-copy
+                    (equal (,length$a (,copy ,%vector ,vector))
+                           (,length$a ,vector))
+                    :hints
+                    (("Goal"
+                      :by (:functional-instance
+                           lem-vector$a::length/resizable-of-copy/resizable
+                           ,@fi-bindings-with-copy))))))
 
          (in-theory
-           (disable ,copy))
+           (disable ,copy-rec
+                    ,copy))
 
          (defthm ,copy{rewrite}
            ,(if element-coupled-p
-                `(implies (case-split (,coupledp ,vector))
+                `(implies (,coupledp ,vector)
                           (equal (,copy ,%vector ,vector)
                                  (,fixer ,vector)))
                 `(equal (,copy ,%vector ,vector)
                         (,fixer$a ,vector)))
            :hints
            (("Goal"
-             :use ((:instance ,vector$a-equal
-                              (,%vector$a (,copy ,%vector ,vector))
-                              (,vector$a (,fixer$a ,vector))))))))
+             :by (:functional-instance
+                  ,(if resizable
+                       'lem-vector$a::copy/resizable{rewrite}
+                       'lem-vector$a::copy/fixed{rewrite})
+                  ,@fi-bindings-with-copy)))))
 
        (deflabel ,coupledp-end)
 
@@ -571,6 +423,8 @@
          (set-difference-theories (current-theory ',coupledp-end)
                                   (current-theory ',coupledp-begin))))))
 
+
+;;;; `MAKE-HASH-TABLE-COPY-EVENTS'
 (defun make-hash-table-copy-events (hash-table state)
   (declare (xargs :stobjs state
                   :guard (symbolp hash-table)
@@ -712,46 +566,10 @@
     `(progn
        (deflabel ,coupledp-begin)
 
-       (encapsulate ()
+       (with-books (("../lemmas/hash-table$a"))
 
          (local
            (deflabel prologue-begin))
-
-         (local
-           (defthm head-not-in-tail
-             (implies (and (not (set::emptyp set))
-                           (equal head (set::head set))
-                           (equal tail (set::tail set)))
-                      (not (set::in head tail)))))
-
-         (local
-           (defthm head-in-set
-             (implies (and (not (set::emptyp set))
-                           (equal head (set::head set)))
-                      (set::in head set))))
-
-         (local
-           (defthm in-tail-iff
-             (implies (and (not (set::emptyp set))
-                           (not (equal element (set::head set))))
-                      (equal (set::in element (set::tail set))
-                             (set::in element set)))
-             :hints
-             (("Goal"
-               :expand (set::in element set)))))
-
-         (local
-           (defthm head-of-tail-neq-head
-             (implies (and (not (set::emptyp set))
-                           (not (set::emptyp (set::tail set))))
-                      (not (equal (set::head (set::tail set))
-                                  (set::head set))))
-             :hints
-             (("Goal"
-               :in-theory (enable set::setp
-                                  set::emptyp
-                                  set::head
-                                  set::tail)))))
 
          ,@(and key-recognizer
                 key-fixer
@@ -801,11 +619,9 @@
          (local
            (in-theory
              (union-theories
-              (union-theories
-               (union-theories (theory 'acl2::ground-zero)
-                               (theory 'set::theorems))
-               (union-theories (theory ',hash-table$a-theorems)
-                               (theory ',hash-table$a-aggressive)))
+              (union-theories (theory 'acl2::ground-zero)
+                              (union-theories (theory ',hash-table$a-theorems)
+                                              (theory ',hash-table$a-aggressive)))
               (set-difference-theories (current-theory 'prologue-end)
                                        (current-theory 'prologue-begin)))))
 
@@ -840,10 +656,6 @@
 
          (local
            (in-theory
-             (acl2::enable* set::expensive-rules)))
-
-         (local
-           (in-theory
              (enable ,@(strip-cars (cdr (getpropc hash-table 'acl2::absstobj-info))))))
 
          (define-congruent ,hash-table)
@@ -864,86 +676,10 @@
                          `(,boundp$a ,key ,hash-table))))
            :rewrite :direct)
 
-         (defthm ,coupled-keys-p-when-not-recognizer$a
-           (implies (not (,recognizer$a ,hash-table))
-                    (,coupled-keys-p ,hash-table)))
-
-         (defthm ,coupled-keys-p-of-creator$a
-           (,coupled-keys-p (,creator$a)))
-
-         (defthm ,coupled-keys-p-of-fixer$a
-           (equal (,coupled-keys-p (,fixer$a ,hash-table))
-                  (,coupled-keys-p ,hash-table)))
-
-         (defthm ,coupled-keys-p-of-updater$a-when-boundp$a
-           (implies (and (,boundp$a ,key ,hash-table)
-                         (,coupled-keys-p ,hash-table))
-                    (,coupled-keys-p (,updater$a ,key ,val ,hash-table))))
-
-         (defthm ,coupled-keys-p-of-updater$a-when-not-boundp$a
-           (implies (let* ((,keys$a (,keys$a ,hash-table))
-                           (trimmed (set::delete ,(if key-fixer
-                                                      `(,key-fixer ,key)
-                                                      key)
-                                                 ,keys$a)))
-                      (and (not (,boundp$a ,key ,hash-table))
-                           (set::in ,(if key-fixer
-                                         `(,key-fixer ,key)
-                                         key)
-                                    ,keys$a)
-                           (,coupled-keys-p (,keys-set$a trimmed ,hash-table))))
-                    (,coupled-keys-p (,updater$a ,key ,val ,hash-table)))
-           :hints
-           (("Goal"
-             :do-not-induct t
-             :in-theory (disable ,coupled-keys-p
-                                 ,coupled-keys-p-necc)
-             :use ((:instance ,coupled-keys-p-necc
-                              (,key (,coupled-keys-p-witness (,updater$a ,default-key ,val ,hash-table)))
-                              (,hash-table (,keys-set$a (set::delete ,default-key (,keys$a ,hash-table))
-                                                        ,hash-table)))
-                   (:instance ,coupled-keys-p-necc
-                              (,key (,coupled-keys-p-witness (,updater$a ,key ,val ,hash-table)))
-                              (,hash-table (,keys-set$a (set::delete k (,keys$a ,hash-table))
-                                                        ,hash-table))))
-             :expand (:free (,key) (,coupled-keys-p (,updater$a ,key ,val ,hash-table))))))
-
-         (defthm ,coupled-keys-p-of-remover$a-when-boundp$a
-           (implies (let* ((,keys$a (,keys$a ,hash-table))
-                           (inserted (set::insert ,(if key-fixer
-                                                       `(,key-fixer ,key)
-                                                       key)
-                                                  ,keys$a)))
-                      (and (,boundp$a ,key ,hash-table)
-                           (not (set::in ,(if key-fixer
-                                              `(,key-fixer ,key)
-                                              key)
-                                         ,keys$a))
-                           (,coupled-keys-p (,keys-set$a inserted ,hash-table))))
-                    (,coupled-keys-p (,remover$a ,key ,hash-table)))
-           :hints
-           (("Goal"
-             :do-not-induct t
-             :in-theory (disable ,coupled-keys-p
-                                 ,coupled-keys-p-necc)
-             :use ((:instance ,coupled-keys-p-necc
-                              (,key (,coupled-keys-p-witness (,remover$a ,default-key ,hash-table)))
-                              (,hash-table (,keys-set$a (set::insert ,default-key (,keys$a ,hash-table))
-                                                        ,hash-table)))
-                   (:instance ,coupled-keys-p-necc
-                              (,key (,coupled-keys-p-witness (,remover$a ,key ,hash-table)))
-                              (,hash-table (,keys-set$a (set::insert ,key (,keys$a ,hash-table))
-                                                        ,hash-table))))
-             :expand (:free (,key) (,coupled-keys-p (,remover$a ,key ,hash-table))))))
-
-         (defthm ,coupled-keys-p-of-remover$a-when-not-boundp$a
-           (implies (and (not (,boundp$a ,key ,hash-table))
-                         (,coupled-keys-p ,hash-table))
-                    (,coupled-keys-p (,remover$a ,key ,hash-table))))
-
          (in-theory
            (disable ,coupled-keys-p))
 
+         ;; `COUPLED-VALS-P'
          ,@(and val-coupled-p
                 `((defun-sk ,coupled-vals-p (,hash-table)
                     (declare (xargs :guard (,recognizer ,hash-table)
@@ -952,61 +688,10 @@
                       (,val-coupled-p (,accessor$a ,key ,hash-table)))
                     :rewrite :direct)
 
-                  (defthm ,coupled-vals-p-when-not-recognizer$a
-                    (implies (not (,recognizer$a ,hash-table))
-                             (,coupled-vals-p ,hash-table)))
-
-                  (defthm ,coupled-vals-p-of-creator$a
-                    (,coupled-vals-p (,creator$a)))
-
-                  (defthm ,coupled-vals-p-of-fixer$a
-                    (equal (,coupled-vals-p (,fixer$a ,hash-table))
-                           (,coupled-vals-p ,hash-table)))
-
-                  (defthm ,coupled-vals-p-of-updater$a
-                    (implies (,coupled-vals-p ,hash-table)
-                             (equal (,coupled-vals-p (,updater$a ,key ,val ,hash-table))
-                                    (,val-coupled-p ,val)))
-                    :hints
-                    (("Goal"
-                      :in-theory (disable ,coupled-vals-p
-                                          ,coupled-vals-p-necc)
-                      :use ((:instance ,coupled-vals-p-necc
-                                       (,hash-table (,updater$a ,key ,val ,hash-table))))
-                      :expand (:free (,key ,val)
-                                     (,coupled-vals-p (,updater$a ,key ,val ,hash-table))))))
-
-                  (defthm ,coupled-vals-p-of-remover$a
-                    (implies (,coupled-vals-p ,hash-table)
-                             (,coupled-vals-p (,remover$a ,key ,hash-table))))
-
-                  (local
-                    (defthmd ,coupled-vals-p-of-keys-set$a-lemma
-                      (iff (,coupled-vals-p (,keys-set$a ,keys$a ,hash-table))
-                           (,coupled-vals-p ,hash-table))
-                      :hints
-                      (("Goal"
-                        :in-theory (disable ,coupled-vals-p
-                                            ,coupled-vals-p-necc))
-                       ("Subgoal 2"
-                        :expand (:free (,keys$a)
-                                       (,coupled-vals-p (,keys-set$a ,keys$a ,hash-table))))
-                       ("Subgoal 1"
-                        :use ((:instance ,coupled-vals-p-necc
-                                         (,key (,coupled-vals-p-witness ,hash-table))
-                                         (,hash-table (,keys-set$a ,keys$a ,hash-table))))
-                        :expand (,coupled-vals-p ,hash-table)))))
-
-                  (defthm ,coupled-vals-p-of-keys-set$a
-                    (equal (,coupled-vals-p (,keys-set$a ,keys$a ,hash-table))
-                           (,coupled-vals-p ,hash-table))
-                    :hints
-                    (("Goal"
-                      :use ,coupled-vals-p-of-keys-set$a-lemma)))
-
                   (in-theory
                     (disable ,coupled-vals-p))))
 
+         ;; `COUPLEDP'
          (defun-nx ,coupledp (,hash-table)
            (declare (xargs :guard (,recognizer ,hash-table)
                            :verify-guards nil))
@@ -1020,14 +705,43 @@
 
          (defthm ,coupledp-when-not-recognizer$a
            (implies (not (,recognizer$a ,hash-table))
-                    (,coupledp ,hash-table)))
+                    (,coupledp ,hash-table))
+           :hints
+           (("Goal"
+             :by (:functional-instance
+                  lem-hash-table$a::coupledp-when-not-recognizer/copyable
+                  ,@fi-bindings))))
 
          (defthm ,coupledp-of-creator$a
-           (,coupledp (,creator$a)))
+           (,coupledp (,creator$a))
+           :hints
+           (("Goal"
+             :by (:functional-instance
+                  lem-hash-table$a::coupledp-of-creator/copyable
+                  ,@fi-bindings))))
 
          (defthm ,coupledp-of-fixer$a
            (equal (,coupledp (,fixer$a ,hash-table))
-                  (,coupledp ,hash-table)))
+                  (,coupledp ,hash-table))
+           :hints
+           (("Goal"
+             :by (:functional-instance
+                  lem-hash-table$a::coupledp-of-fixer/copyable
+                  ,@fi-bindings))))
+
+         ,@(and val-coupled-p
+                `((defthm ,val-coupled-p-of-accessor$a
+                    (implies (,coupledp ,hash-table)
+                             (,val-coupled-p (,accessor$a ,key ,hash-table)))
+                    :rule-classes
+                    ((:rewrite :corollary
+                               (implies (coupledp ,hash-table)
+                                        (,val-coupled-p (,accessor$a ,key ,hash-table)))))
+                    :hints
+                    (("Goal"
+                      :by (:functional-instance
+                           lem-hash-table$a::val-coupled-p-of-accessor/copyable
+                           ,@fi-bindings))))))
 
          (defthm ,coupledp-of-updater$a-when-boundp$a
            (implies (and (,boundp$a ,key ,hash-table)
@@ -1035,269 +749,199 @@
                     ,(if val-coupled-p
                          `(equal (,coupledp (,updater$a ,key ,val ,hash-table))
                                  (,val-coupled-p ,val))
-                         `(,coupledp (,updater$a ,key ,val ,hash-table)))))
+                         `(,coupledp (,updater$a ,key ,val ,hash-table))))
+           :hints
+           (("Goal"
+             :by (:functional-instance
+                  lem-hash-table$a::coupledp-of-updater/copyable-when-boundp/copyable
+                  ,@fi-bindings))))
 
          (defthm ,coupledp-of-updater$a-when-not-boundp$a
            (implies (let* ((,keys$a (,keys$a ,hash-table))
-                           (trimmed (set::delete ,(if key-fixer
-                                                      `(,key-fixer ,key)
-                                                      key)
-                                                 ,keys$a)))
+                           (trimmed (set::delete ,(if key-fixer `(,key-fixer ,key) key) ,keys$a)))
                       (and (not (,boundp$a ,key ,hash-table))
-                           (set::in ,(if key-fixer
-                                         `(,key-fixer ,key)
-                                         key)
-                                    ,keys$a)
+                           (set::in ,(if key-fixer `(,key-fixer ,key) key) ,keys$a)
                            (,coupledp (,keys-set$a trimmed ,hash-table))))
                     ,(if val-coupled-p
                          `(equal (,coupledp (,updater$a ,key ,val ,hash-table))
                                  (,val-coupled-p ,val))
-                         `(,coupledp (,updater$a ,key ,val ,hash-table)))))
+                         `(,coupledp (,updater$a ,key ,val ,hash-table))))
+           :hints
+           (("Goal"
+             :by (:functional-instance
+                  lem-hash-table$a::coupledp-of-updater/copyable-when-not-boundp/copyable
+                  ,@fi-bindings))))
 
-         (defthm ,coupledp-of-remover$a-when-boundp$a
-           (implies (let* ((,keys$a (,keys$a ,hash-table))
-                           (inserted (set::insert ,(if key-fixer
-                                                       `(,key-fixer ,key)
-                                                       key)
-                                                  ,keys$a)))
-                      (and (,boundp$a ,key ,hash-table)
-                           (not (set::in ,(if key-fixer
-                                              `(,key-fixer ,key)
-                                              key)
-                                         ,keys$a))
-                           (,coupledp (,keys-set$a inserted ,hash-table))))
-                    (,coupledp (,remover$a ,key ,hash-table))))
-
-         (defthm ,coupledp-of-remover$a-when-not-boundp$a
-           (implies (and (not (,boundp$a ,key ,hash-table))
-                         (,coupledp ,hash-table))
-                    (,coupledp (,remover$a ,key ,hash-table))))
-
-         (defthm ,cardinality-of-keys$a
-           (implies (,coupledp ,hash-table)
-                    (equal (set::cardinality (,keys$a ,hash-table))
-                           (,count$a ,hash-table))))
-
-         (defthm ,in-of-keys$a
+         (defthm ,in-of-keys$a-when-coupledp
            (implies (,coupledp ,hash-table)
                     (equal (set::in ,key (,keys$a ,hash-table))
                            ,(if key-recognizer
                                 `(and (,key-recognizer ,key)
                                       (,boundp$a ,key ,hash-table))
-                                `(,boundp$a ,key ,hash-table)))))
+                                `(,boundp$a ,key ,hash-table))))
+           :hints
+           (("Goal"
+             :by (:functional-instance
+                  lem-hash-table$a::in-of-keys-when-coupledp
+                  ,@fi-bindings))))
 
-         ,@(and val-coupled-p
-                `((defthm ,val-coupled-p-of-accessor$a
-                    (implies (,coupledp ,hash-table)
-                             (,val-coupled-p (,accessor$a ,key ,hash-table))))))
+         (defthm ,coupledp-of-remover$a-when-boundp$a
+           (implies (let* ((,keys$a (,keys$a ,hash-table))
+                           (inserted (set::insert ,(if key-fixer `(,key-fixer ,key) key) ,keys$a)))
+                      (and (,boundp$a ,key ,hash-table)
+                           (not (set::in ,(if key-fixer `(,key-fixer ,key) key) ,keys$a))
+                           (,coupledp (,keys-set$a inserted ,hash-table))))
+                    (,coupledp (,remover$a ,key ,hash-table)))
+           :hints
+           (("Goal"
+             :by (:functional-instance
+                  lem-hash-table$a::coupledp-of-remover/copyable-when-boundp/copyable
+                  ,@fi-bindings))))
 
-         (defthm ,emptyp-of-keys$a
+         (defthm ,coupledp-of-remover$a-when-not-boundp$a
+           (implies (and (not (,boundp$a ,key ,hash-table))
+                         (,coupledp ,hash-table))
+                    (,coupledp (,remover$a ,key ,hash-table)))
+           :hints
+           (("Goal"
+             :by (:functional-instance
+                  lem-hash-table$a::coupledp-of-remover/copyable-when-not-boundp/copyable
+                  ,@fi-bindings))))
+
+         (defthm ,cardinality-of-keys$a-when-coupledp
+           (implies (,coupledp ,hash-table)
+                    (equal (set::cardinality (,keys$a ,hash-table))
+                           (,count$a ,hash-table)))
+           :hints
+           (("Goal"
+             :by (:functional-instance
+                  lem-hash-table$a::cardinality-of-keys-when-coupledp
+                  ,@fi-bindings))))
+
+         (defthm ,emptyp-of-keys$a-when-coupledp
            (implies (,coupledp ,hash-table)
                     (equal (set::emptyp (,keys$a ,hash-table))
-                           (= (,count$a ,hash-table) 0))))
+                           (or (not (,recognizer$a ,hash-table))
+                               (equal ,hash-table (,creator$a)))))
+           :hints
+           (("Goal"
+             :by (:functional-instance
+                  lem-hash-table$a::emptyp-of-keys-when-coupledp
+                  ,@fi-bindings))))
 
          (in-theory
            (disable ,coupledp))
 
+         ;; `COPY-REC'
          (defun ,copy-rec (set ,%hash-table ,hash-table)
            (declare (xargs :stobjs (,%hash-table ,hash-table)
                            :guard (and (,keysp$a set)
                                        (set::subset set (,keys ,hash-table)))))
-           ,(let ((body
-                   `(if (set::emptyp set)
-                        ;; TODO: replace above condition with (set::emptyp
-                        ;; (,keys$a-fix set)) for performance and remove let
-                        ;; wrapper.
-                        (,fixer ,%hash-table)
-                        ,(if val-copy
-                             `(let ((,key ,(if key-fixer
-                                               `(,key-fixer (set::head set))
-                                               '(set::head set))))
-                                (stobj-let ((,val (,accessor ,key ,hash-table) ,updater))
-                                           (,%hash-table)
-                                           (stobj-let ((,%val (,%accessor ,key ,%hash-table) ,%updater))
-                                                      (,%val)
-                                                      (,val-copy ,%val ,val)
-                                             ,%hash-table)
-                                  (,copy-rec (set::tail set) ,%hash-table ,hash-table)))
-                             `(let* ((,key (set::head set))
-                                     (,val (,accessor ,key ,hash-table))
-                                     (,%hash-table (,updater ,key ,val ,%hash-table)))
-                                (,copy-rec (set::tail set) ,%hash-table ,hash-table))))))
-              (if key-recognizer
-                  `(let ((set (,keys$a-fix set)))
-                     ,body)
-                  body)))
+           (if (set::emptyp set)
+               (,fixer ,%hash-table)
+               ,(if val-copy
+                    `(let ((,key ,(if key-fixer `(,key-fixer (set::head set)) '(set::head set))))
+                       (stobj-let ((,val (,accessor ,key ,hash-table) ,updater))
+                                  (,%hash-table)
+                                  (stobj-let ((,%val (,%accessor ,key ,%hash-table) ,%updater))
+                                             (,%val)
+                                             (,val-copy ,%val ,val)
+                                    ,%hash-table)
+                         (,copy-rec (set::tail set) ,%hash-table ,hash-table)))
+                    `(let* ((,key ,(if key-fixer `(,key-fixer (set::head set)) '(set::head set)))
+                            (,val (,accessor ,key ,hash-table))
+                            (,%hash-table (,updater ,key ,val ,%hash-table)))
+                       (,copy-rec (set::tail set) ,%hash-table ,hash-table)))))
 
-         (local
-           (defthm ,recognizer$a-of-copy-rec
-             (,recognizer$a (,copy-rec set ,%hash-table ,hash-table))))
-
-         (local
-           (defthm ,keys$a-of-copy-rec
-             (equal (,keys$a (,copy-rec set ,%hash-table ,hash-table))
-                    (,keys$a ,%hash-table))))
-
-         (local
-           (defthm ,copy-rec-of-updater$a
-             (implies (and (,coupledp ,hash-table)
-                           (set::subset set (,keys$a ,hash-table)))
-                      (equal (,copy-rec set (,updater$a ,key ,val ,%hash-table) ,hash-table)
-                             (if (set::in ,(if key-fixer
-                                               `(,key-fixer ,key)
-                                               key)
-                                          set)
-                                 (,copy-rec set ,%hash-table ,hash-table)
-                                 (,updater$a ,key ,val (,copy-rec set ,%hash-table ,hash-table)))))
-             :hints
-             (("Goal"
-               :induct (,copy-rec set ,%hash-table ,hash-table)
-               :in-theory (enable set::in)
-               :expand (:free (,key)
-                              (,copy-rec set (,updater$a ,key ,val ,%hash-table) ,hash-table)))
-              ("Subgoal *1/1"
-               :cases ((set::emptyp set))))))
-
-         (local
-           (defthm ,boundp$a-of-copy-rec
-             (implies (and (,coupledp ,hash-table)
-                           (set::subset set (,keys$a ,hash-table)))
-                      (equal (,boundp$a ,key (,copy-rec set ,%hash-table ,hash-table))
-                             (or (,boundp$a ,key ,%hash-table)
-                                 (set::in ,(if key-fixer
-                                               `(,key-fixer ,key)
-                                               key)
-                                          set))))
-             :hints
-             (("Goal"
-               :induct (,copy-rec set ,%hash-table ,hash-table)
-               :in-theory (enable set::in))
-              ("Subgoal *1/1"
-               :cases ((set::emptyp set))))))
-
-         (local
-           (defthm ,accessor$a-of-copy-rec
-             (implies (and (,coupledp ,hash-table)
-                           (set::subset set (,keys$a ,hash-table)))
-                      (equal (,accessor$a ,key (,copy-rec set ,%hash-table ,hash-table))
-                             (if (set::in ,(if key-fixer
-                                               `(,key-fixer ,key)
-                                               key)
-                                          set)
-                                 (,accessor$a ,key ,hash-table)
-                                 (,accessor$a ,key ,%hash-table))))
-             :hints
-             (("Goal"
-               :induct (,copy-rec set ,%hash-table ,hash-table)
-               :in-theory (enable set::in)))))
-
-         (local
-           (defthm ,count$a-of-copy-rec
-             (implies (and (,coupledp ,hash-table)
-                           (set::subset set (,keys$a ,hash-table)))
-                      (equal (,count$a (,copy-rec set ,%hash-table ,hash-table))
-                             (cond
-                               (,(if key-recognizer
-                                     `(or (set::emptyp set)
-                                          (not (,keysp$a set)))
-                                     `(set::emptyp set))
-                                (,count$a ,%hash-table))
-                               ((,boundp$a (set::head set) ,%hash-table)
-                                (,count$a (,copy-rec (set::tail set) ,%hash-table ,hash-table)))
-                               (t
-                                (1+ (,count$a (,copy-rec (set::tail set) ,%hash-table ,hash-table)))))))))
-
-         (in-theory
-           (disable ,copy-rec))
-
+         ;; `COPY'
          (defun ,copy (,%hash-table ,hash-table)
            (declare (xargs :stobjs (,%hash-table ,hash-table)))
-           (let* ((keys (,keys ,hash-table))
-                  (count (,count ,hash-table))
-                  (,%hash-table (,init count nil nil ,%hash-table))
-                  (,%hash-table (,keys-set keys ,%hash-table)))
+           (let* ((,keys (,keys ,hash-table))
+                  (,count (,count ,hash-table))
+                  (,%hash-table (,init ,count nil nil ,%hash-table))
+                  (,%hash-table (,keys-set ,keys ,%hash-table)))
              (,copy-rec keys ,%hash-table ,hash-table)))
 
          (table copy ',hash-table ',copy)
 
          (defthm ,recognizer$a-of-copy
-           (,recognizer$a (,copy ,%hash-table ,hash-table)))
+           (,recognizer$a (,copy ,%hash-table ,hash-table))
+           :hints
+           (("Goal"
+             :by (:functional-instance
+                  lem-hash-table$a::recognizer/copyable-of-copy
+                  ,@fi-bindings))))
 
-         (local
-           (defthm ,coupledp-of-copy/lemma-0
-             (implies (and (,(if key-recognizer
-                                 keysp$a
-                                 'set::setp)
-                             %set)
-                           (,coupledp ,hash-table)
-                           (set::subset set (,keys$a ,hash-table)))
-                      (equal (,count$a (,copy-rec set (,keys-set$a %set (,creator$a)) ,hash-table))
-                             (,count$a (,copy-rec set (,creator$a) ,hash-table))))
-             :hints
-             (("Goal"
-               :induct (set::cardinality set)
-               :in-theory (enable (:i set::cardinality))))))
+         (defthm ,copy-of-fixer$a-1
+           (equal (,copy (,fixer$a ,%hash-table) ,hash-table)
+                  (,copy ,%hash-table ,hash-table))
+           :hints
+           (("Goal"
+             :by (:functional-instance
+                  lem-hash-table$a::copy-of-fixer/copyable-1
+                  ,@fi-bindings))))
 
-         (local
-           (defthm ,coupledp-of-copy/lemma-1
-             (implies (and (,coupledp ,hash-table)
-                           (set::subset set (,keys$a ,hash-table)))
-                      (equal (,count$a (,copy-rec set (,creator$a) ,hash-table))
-                             (set::cardinality set)))
-             :hints
-             (("Goal"
-               :induct (set::cardinality set)
-               :in-theory (enable set::cardinality)))))
+         (defthm ,copy-of-fixer$a-2
+           (equal (,copy ,%hash-table (,fixer$a ,hash-table))
+                  (,copy ,%hash-table ,hash-table))
+           :hints
+           (("Goal"
+             :by (:functional-instance
+                  lem-hash-table$a::copy-of-fixer/copyable-2
+                  ,@fi-bindings))))
 
-         (local
-           (defthm ,coupledp-of-copy
-             (implies (,coupledp ,hash-table)
-                      (,coupledp (,copy ,%hash-table ,hash-table)))
-             :hints
-             (("Goal"
-               :in-theory (enable ,coupled-keys-p
-                                  ,@(and val-coupled-p
-                                         (list coupled-vals-p)))
-               :expand (:free (set ,%hash-table ,hash-table)
-                              (,coupledp (,copy-rec set ,%hash-table ,hash-table))))
-              ("Subgoal 1"
-               :expand (,coupledp ,hash-table)))))
+         (defthm ,count$a-of-copy
+           (implies (,coupledp ,hash-table)
+                    (equal (,count$a (,copy ,%hash-table ,hash-table))
+                           (,count$a ,hash-table)))
+           :hints
+           (("Goal"
+             :by (:functional-instance
+                  lem-hash-table$a::count/copyable-of-copy
+                  ,@fi-bindings))))
+
+         (defthm ,accessor$a-of-copy
+           (implies (,coupledp ,hash-table)
+                    (equal (,accessor$a ,key (,copy ,%hash-table ,hash-table))
+                           (,accessor$a ,key ,hash-table)))
+           :hints
+           (("Goal"
+             :by (:functional-instance
+                  lem-hash-table$a::accessor/copyable-of-copy
+                  ,@fi-bindings))))
+
+         (defthm ,boundp$a-of-copy
+           (implies (,coupledp ,hash-table)
+                    (equal (,boundp$a ,key (,copy ,%hash-table ,hash-table))
+                           (,boundp$a ,key ,hash-table)))
+           :hints
+           (("Goal"
+             :by (:functional-instance
+                  lem-hash-table$a::boundp/copyable-of-copy
+                  ,@fi-bindings))))
 
          (defthm ,keys$a-of-copy
            (equal (,keys$a (,copy ,%hash-table ,hash-table))
-                  (,keys$a ,hash-table)))
-
-         (local
-           (defthm ,boundp$a-of-copy
-             (implies (,coupledp ,hash-table)
-                      (equal (,boundp$a ,key (,copy ,%hash-table ,hash-table))
-                             (,boundp$a ,key ,hash-table)))))
-
-         (local
-           (defthm ,accessor$a-of-copy
-             (implies (,coupledp ,hash-table)
-                      (equal (,accessor$a ,key (,copy ,%hash-table ,hash-table))
-                             (,accessor$a ,key ,hash-table)))))
-
-         (local
-           (defthm ,count$a-of-copy
-             (implies (,coupledp ,hash-table)
-                      (equal (,count$a (,copy ,%hash-table ,hash-table))
-                             (,count$a ,hash-table)))))
+                  (,keys$a ,hash-table))
+           :hints
+           (("Goal"
+             :by (:functional-instance
+                  lem-hash-table$a::keys-of-copy
+                  ,@fi-bindings))))
 
          (in-theory
-           (disable ,copy))
+           (disable ,copy-rec
+                    ,copy))
 
          (defthm ,copy{rewrite}
-           (implies (case-split (,coupledp ,hash-table))
+           (implies (,coupledp ,hash-table)
                     (equal (,copy ,%hash-table ,hash-table)
                            (,fixer$a ,hash-table)))
            :hints
-           (("goal"
-             :do-not-induct t
-             :use ((:instance ,hash-table$a-equal
-                              (,%hash-table$a (,copy ,%hash-table ,hash-table))
-                              (,hash-table$a (,fixer$a ,hash-table))))))))
+           (("Goal"
+             :by (:functional-instance
+                  lem-hash-table$a::copy{rewrite}
+                  ,@fi-bindings)))))
 
        (deflabel ,coupledp-end)
 
@@ -1305,6 +949,8 @@
          (set-difference-theories (current-theory ',coupledp-end)
                                   (current-theory ',coupledp-begin))))))
 
+
+;;;; `MAKE-FRAME-COPY-EVENTS'
 (defun make-frame-copy-events (stobj$a %stobj stobj state)
   (declare (xargs :stobjs state
                   :guard (and (symbolp stobj$a)
@@ -1532,7 +1178,6 @@
            :use ((:instance ,stobj$a-equal
                             (,%stobj$a (,copier ,%stobj ,stobj))
                             (,stobj$a (,fixer ,stobj))))))))))
-
 
 
 ;;;; `DEFINE-COPY'
